tests/CountBy/CountBy.v
@@ -1,0 +1,76 @@
+(****************************************************************************)
+(* Copyright 2020 The Project Oak Authors                                   *)
+(*                                                                          *)
+(* Licensed under the Apache License, Version 2.0 (the "License")           *)
+(* you may not use this file except in compliance with the License.         *)
+(* You may obtain a copy of the License at                                  *)
+(*                                                                          *)
+(*     http://www.apache.org/licenses/LICENSE-2.0                           *)
+(*                                                                          *)
+(* Unless required by applicable law or agreed to in writing, software      *)
+(* distributed under the License is distributed on an "AS IS" BASIS,        *)
+(* WITHOUT WARRANTIES OR CONDITIONS OF ANY KIND, either express or implied. *)
+(* See the License for the specific language governing permissions and      *)
+(* limitations under the License.                                           *)
+(****************************************************************************)
+
+From Coq Require Import NArith.NArith Lists.List.
+Import ListNotations.
+
+Require Import ExtLib.Structures.Monads.
+Export MonadNotation.
+
+Require Import Cava.Acorn.Identity.
+Require Import Cava.Cava.
+Require Import Cava.Tactics.
+Require Import Cava.Monad.CavaMonad.
+Require Import Cava.Lib.UnsignedAdders.
+
+(******************************************************************************)
+(* countBy                                                                    *)
+(******************************************************************************) 
+
+(*
+
+The countBy circuit takes the current 8-bit input (in) and the current
+state value represented by the register (delay) which is output in the
+current cycle as the output of the circuit, and this value is also the
+next state value for the delay. The adder is an 8-bit adder with no
+bit-growth i.e. it computes (a + b) mod 256.
+
+        _______
+    ---| delay |------------
+   |   |_______|            |
+   |   ___                  |
+    --| + ---------------------- out
+ in --|___|
+
+*)
+
+Section WithCava.
+  Context {signal} {semantics:Cava signal} `{Monad cava}.
+
+  Definition countFork (i : signal (Vec Bit 8) * signal (Vec Bit 8))
+                       : cava (signal (Vec Bit 8) * signal (Vec Bit 8)) :=
+    newCount <- addN (fst i) (snd i) ;;
+    ret (newCount, newCount).
+
+  Definition countBy : signal (Vec Bit 8) -> cava (signal (Vec Bit 8))
+    := loop countFork.
+
+End WithCava.
+
+(* Convenience notations for certain bytes *)
+Definition b0 := N2Bv_sized 8 0.
+Definition b3 := N2Bv_sized 8 3.
+Definition b7 := N2Bv_sized 8 7.
+Definition b14 := N2Bv_sized 8 14.
+Definition b18 := N2Bv_sized 8 18.
+Definition b21 := N2Bv_sized 8 21.
+Definition b24 := N2Bv_sized 8 24.
+Definition b250 := N2Bv_sized 8 250.
+
+Local Open Scope list_scope.
+
+Example countBy_ex1: sequential (countBy [b14; b7; b3; b250]) = [b14; b21; b24; b18].
+Proof. reflexivity. Qed.
