tests/CountBy/ListProofs.v
@@ -1,0 +1,90 @@
+(****************************************************************************)
+(* Copyright 2020 The Project Oak Authors                                   *)
+(*                                                                          *)
+(* Licensed under the Apache License, Version 2.0 (the "License")           *)
+(* you may not use this file except in compliance with the License.         *)
+(* You may obtain a copy of the License at                                  *)
+(*                                                                          *)
+(*     http://www.apache.org/licenses/LICENSE-2.0                           *)
+(*                                                                          *)
+(* Unless required by applicable law or agreed to in writing, software      *)
+(* distributed under the License is distributed on an "AS IS" BASIS,        *)
+(* WITHOUT WARRANTIES OR CONDITIONS OF ANY KIND, either express or implied. *)
+(* See the License for the specific language governing permissions and      *)
+(* limitations under the License.                                           *)
+(****************************************************************************)
+
+From Coq Require Import NArith.NArith Lists.List.
+Require Import Coq.Bool.Bvector.
+Import ListNotations.
+
+Require Import ExtLib.Structures.Monads.
+Export MonadNotation.
+
+Require Import Cava.Acorn.Identity.
+Require Import Cava.Cava.
+Require Import Cava.Tactics.
+Require Import Cava.Monad.CavaMonad.
+Require Import Cava.Lib.UnsignedAdders.
+
+Require Import Tests.CountBy.CountBy.
+
+Fixpoint countBySpec' (state: Bvector 8) (i : list (Bvector 8))
+                      : list (Bvector 8) :=
+  match i with
+  | [] => []
+  | x::xs =>
+    let newState := N2Bv_sized 8 (Bv2N x + Bv2N state) in
+    newState :: countBySpec' newState xs
+  end.
+
+Definition countBySpec := countBySpec' (N2Bv_sized 8 0).
+
+(* TODO: addN sequential seems to only return one result; shouldn't it be a map2? *)
+Definition addNSpec {n} (a b : list (Bvector n)) : list (Bvector n) :=
+  match a,b with
+  | a :: _, b :: _ => [N2Bv_sized n ((Bv2N a + Bv2N b))]
+  | _,_ => []
+  end.
+
+Local Ltac seqsimpl_step :=
+  first [ progress cbn beta iota delta
+                   [fst snd hd sequential loopSeq' loop SequentialCombSemantics]
+        | progress cbv beta iota delta [loopSeq]; seqsimpl_step
+        | progress autorewrite with seqsimpl
+        | progress destruct_pair_let
+        | progress simpl_ident ].
+Local Ltac seqsimpl := repeat seqsimpl_step.
+
+(* TODO: rename typeclass arguments *)
+Lemma addNCorrect n (a b : list (Bvector n)) :
+  sequential (addN (H:=SequentialCombSemantics) a b) = addNSpec a b.
+Admitted.
+Hint Rewrite addNCorrect using solve [eauto] : seqsimpl.
+
+Lemma countForkStep:
+  forall (i : Bvector 8) (s : Bvector 8),
+    sequential (countFork (semantics:=SequentialCombSemantics) ([i], [s]))
+    = (countBySpec' s [i], countBySpec' s [i]).
+Proof.
+  intros; cbv [countFork countBySpec'].
+  seqsimpl; reflexivity.
+Qed.
+Hint Rewrite countForkStep using solve [eauto] : seqsimpl.
+
+Lemma countForkCorrect:
+  forall (i : list (Bvector 8)) (s : Bvector 8),
+    sequential (loopSeq' (countFork (semantics:=SequentialCombSemantics)) i [s])
+    = countBySpec' s i.
+Proof.
+  cbv [sequential]; induction i; intros; [ reflexivity | ].
+  seqsimpl. cbn [countBySpec']; rewrite IHi; reflexivity.
+Qed.
+Hint Rewrite countForkCorrect using solve [eauto] : seqsimpl.
+
+Lemma countByCorrect: forall (i : list (Bvector 8)),
+                      sequential (countBy i) = countBySpec i.
+Proof.
+  intros; cbv [countBy countBySpec].
+  seqsimpl; reflexivity.
+Qed.
